theories/Constr/MapUpdate.v
@@ -523,3 +523,32 @@ Proof.
       * invt NoDupA.
         eexists x0. lud; eauto. cset_tac.
 Qed.
+
+Set Implicit Arguments.
+
+Section MapUpdate'.
+  Open Scope fmap_scope.
+  Variable X : Type.
+  Context `{OrderedType X}.
+  Variable Y : Type.
+
+  Fixpoint update_with_list' XL YL (m:X -> Y) :=
+    match XL, YL with
+      | x::XL, y::YL => update_with_list' XL YL (m[x <- y])
+      | _, _ => m
+    end.
+
+  Lemma update_with_list_agree' (XL:list X) (VL:list Y) E D
+  : length XL = length VL
+    -> NoDupA _eq XL
+    -> agree_on eq D (E [XL <-- VL]) (update_with_list' XL VL E).
+  Proof.
+    intros LEN UNIQ. length_equify.
+    general induction LEN; simpl in *; eauto.
+    - etransitivity. symmetry.
+      eapply update_nodup_commute_eq; eauto using length_eq_length.
+      eapply IHLEN; eauto.
+  Qed.
+End MapUpdate'.
+
+Notation "f [ w <-/- x ]" := (update_with_list' w x f) (at level 29, left associativity).
